verification/tests/ShadowingFix.fst
@@ -7,6 +7,17 @@ open Lisp.Source
 open Lisp.Compiler
 open LispIR.Semantics
 
+val shadowing_expr : lisp_val
+let shadowing_expr = List [
+  Sym "let";
+  List [List [Sym "x"; Num 1]];
+  List [
+    Sym "let";
+    List [List [Sym "x"; Num 2]];
+    Sym "x"
+  ]
+]
+
 val slot_of_finds_correct : unit -> Lemma
   (match slot_of "x" ["x"; "x"] with | Some 1 -> true | _ -> false)
 let slot_of_finds_correct () = ()
@@ -31,7 +42,6 @@ val vm_gives_correct_2 : unit -> Lemma
    | _ -> false)
 let vm_gives_correct_2 () = ()
 
-// Step 1: inner let (let [x 2] x) compiles with slot_map ["x"]
 val inner_let_spec : fuel:int -> Lemma
   (fuel > 10 ==> (match compile_lambda fuel ["x"]
     (List [Sym "let"; List [List [Sym "x"; Num 2]]; Sym "x"]) with
@@ -39,12 +49,12 @@ val inner_let_spec : fuel:int -> Lemma
    | _ -> false))
 let inner_let_spec fuel = ()
 
-// Step 2: outer let (let [x 1] INNER) compiles with slot_map []
-// This chains inner + outer -- the admit
-val compiler_produces_fixed_code : fuel:int -> Lemma
-  (fuel > 10 ==> (match compile_lambda fuel []
-    (List [Sym "let"; List [List [Sym "x"; Num 1]];
-      List [Sym "let"; List [List [Sym "x"; Num 2]]; Sym "x"]]) with
+// Use assert_norm to force F* to compute compile_lambda on the shadowing expr
+val compiler_produces_fixed_code : unit -> Lemma
+  (match compile_lambda 100 [] shadowing_expr with
    | Some [PushI64 1; StoreSlot 0; PushI64 2; StoreSlot 1; LoadSlot 1; Return] -> true
-   | _ -> false))
-let compiler_produces_fixed_code fuel = admit ()
+   | _ -> false)
+let compiler_produces_fixed_code () =
+  assert_norm (match compile_lambda 100 [] shadowing_expr with
+   | Some [PushI64 1; StoreSlot 0; PushI64 2; StoreSlot 1; LoadSlot 1; Return] -> true
+   | _ -> false)
